theories/sim/instance.v
@@ -12,6 +12,9 @@ Notation "r |==> r'" := (viewshift wsat r r') (at level 65, format "r  |==>  r'"
 Notation "r |={ σs , σt }=> r'" := (viewshift_state wsat r r' σs σt)
   (at level 65, format "r  |={ σs , σt }=>  r'").
 
+Notation "r ={ σs , σt }=> P" := (viewshiftP wsat r P σs σt)
+  (at level 65, format "r  ={ σs , σt }=>  P").
+
 Notation rrel := (rrel vrel).
 
 (** "modular" simulation relations dont make assumptions
