theories/sim/left_step.v
@@ -1,7 +1,7 @@
 From iris.algebra Require Import local_updates.
 
 From stbor.lang Require Import steps_progress steps_inversion steps_retag.
-From stbor.sim Require Export instance.
+From stbor.sim Require Export instance invariant_access body.
 
 Set Default Proof Using "Type".
 
@@ -53,16 +53,89 @@ Proof.
 Qed.
 
 Lemma sim_body_copy_unique_l
-  fs ft (r r': resUR) (h: heaplet) n (l: loc) tg T (s: scalar) et σs σt Φ :
+  fs ft (r r': resUR) (h: heaplet) n (l: loc) t T (s: scalar) et σs σt Φ :
   tsize T = 1%nat →
-  r ≡ r' ⋅ res_tag tg tkUnique h →
+  r ≡ r' ⋅ res_tag t tkUnique h →
   h !! l = Some s →
   (r ⊨{n,fs,ft} (#[s], σs) ≥ (et, σt) : Φ : Prop) →
-  r ⊨{n,fs,ft} (Copy (Place l (Tagged tg) T), σs) ≥ (et, σt) : Φ.
+  r ⊨{n,fs,ft} (Copy (Place l (Tagged t) T), σs) ≥ (et, σt) : Φ.
 Proof.
+  intros LenT Eqr Eqs CONT. pfold. intros NT. intros.
+  have WSAT1 := WSAT. (* backup *)
+
+  (* making a step *)
+  edestruct (NT (Copy (Place l (Tagged t) T)) σs) as [[]|[es' [σs' STEPS]]];
+    [done..|].
+  destruct (tstep_copy_inv _ (PlaceR _ _ _) _ _ _ STEPS)
+      as (l'&t'&T'& vs & α' & EqH & ? & Eqvs & Eqα' & ?).
+  symmetry in EqH. simplify_eq.
+
+  rewrite LenT read_mem_equation_1 /= in Eqvs.
+  destruct (σs.(shp) !! l) as [s'|] eqn:Eqs'; [|done].
+  simpl in Eqvs. simplify_eq.
+
+  destruct WSAT as (WFS & WFT & VALID & PINV & CINV & SREL & LINV).
+  (* some lookup properties *)
+  have VALIDr := cmra_valid_op_r _ _ VALID. rewrite ->Eqr in VALIDr.
+  have HLtr: r.(rtm) !! t ≡ Some (to_tagKindR tkUnique, to_agree <$> h).
+  { rewrite Eqr.
+    eapply tmap_lookup_op_unique_included;
+      [apply VALIDr|apply cmra_included_r|].
+    rewrite res_tag_lookup //. }
+  have HLtrf: (r_f ⋅ r).(rtm) !! t ≡ Some (to_tagKindR tkUnique, to_agree <$> h).
+  { apply tmap_lookup_op_r_unique_equiv; [apply VALID|done]. }
+
+  (* Unique: stack unchanged *)
+  destruct (for_each_lookup_case_2 _ _ _ _ _ Eqα') as [EQ1 _].
+  specialize (EQ1 O) as (stk & stk' & Eqstk & Eqstk' & ACC1); [rewrite LenT; lia|].
+  rewrite shift_loc_0_nat in Eqstk, Eqstk'.
+  move : ACC1. case access1 as [[n1 stk1]|] eqn:ACC1; [|done].
+  simpl. intros Eqs1. symmetry in Eqs1. simplify_eq.
+
+  destruct SREL as (Eqst&Eqnp&Eqcs&Eqnc&AREL).
+  rewrite Eqst in Eqstk. rewrite Eqcs in ACC1.
+
+  destruct (unique_access_head _ _ _ _ _ _ _ _ s _ Eqstk ACC1 PINV HLtrf)
+    as (it & Eqpit & Eqti & HDi & Eqhp); [by rewrite lookup_fmap Eqs |].
+
+  have ?: α' = σt.(sst).
+  { move : Eqα'.
+    rewrite LenT /= /memory_read /= /= shift_loc_0_nat Eqst Eqstk /= Eqcs ACC1 /=.
+    destruct (tag_unique_head_access σt.(scs) stk (Tagged t) it.(protector) AccessRead)
+      as [ns Eqss].
+    - destruct HDi as [stk' Eq']. exists stk'. rewrite Eq'. f_equal.
+      rewrite -Eqpit -Eqti. by destruct it.
+    - rewrite ACC1 in Eqss. simplify_eq. rewrite insert_id //. by inversion 1. }
+  subst α'. rewrite Eqstk in Eqstk'. symmetry in Eqstk'. simplify_eq.
+
+  have TOT: tag_on_top σt.(sst) l t.
+  { destruct HDi as [stk' Eqstk'].
+    rewrite /tag_on_top Eqstk Eqstk' /= -Eqpit -Eqti. destruct it. by eexists. }
+
+  rewrite (_: mkState σs.(shp) σt.(sst) σs.(scs) σs.(snp) σs.(snc) = σs) in STEPS;
+    last first. { rewrite -Eqst. by destruct σs. }
+
+  (* we read s' from σs(l), we know [s] is in σt(l), now we have to prove that
+    s' = s *)
+  assert (s' = s). { admit. } subst s'.
+
+  have STEPSS: (Copy (Place l (Tagged t) T), σs) ~{fs}~>* (#[s]%E, σs)
+    by apply rtc_once.
+  have NT' := never_stuck_tstep_once _ _ _ _ _ STEPS NT.
+  (* TODO: the following is the same in most proofs, generalize it *)
+  punfold CONT. specialize (CONT NT' _ WSAT1) as [RE TE ST]. split; [done|..].
+  - intros. specialize (TE _ TERM) as (vs' & σs' & r1 & STEPS' & POST).
+    exists vs', σs', r1. split; [|done]. etrans; eauto.
+  - inversion ST.
+    + constructor 1. intros.
+      destruct (STEP _ _ STEPT) as (es' & σs' & r1 & n' & STEPS' & POST).
+      exists es', σs', r1, n'. split; [|done].
+      left. destruct STEPS' as [?|[]].
+      * eapply tc_rtc_l; eauto.
+      * simplify_eq. by apply tc_once.
+    + econstructor 2; eauto. by etrans.
 Admitted.
 
-(* should be a fairly direct consequence of the above *)
 Lemma sim_body_copy_local_l fs ft r r' n l tg ty s et σs σt Φ :
   tsize ty = 1%nat →
   r ≡ r' ⋅ res_mapsto l [s] tg →
@@ -71,6 +144,9 @@ Lemma sim_body_copy_local_l fs ft r r' n l tg ty s et σs σt Φ :
     (Copy (Place l (Tagged tg) ty), σs) ≥ (et, σt)
   : Φ.
 Proof.
-Admitted.
+  intros Hty Hr. rewrite Hr cmra_assoc. intros CONT.
+  eapply sim_body_copy_unique_l; eauto.
+  by rewrite lookup_insert.
+Qed.
 
 End left.
